Link v_G, v_H, and v_PRF with spec

libcrux-ml-kem/src/hash_functions.rs
@@ -67,6 +67,9 @@ pub(crate) mod portable {
         shake128_state: [KeccakState; K],
     }
 
+    #[cfg_attr(hax,hax_lib::ensures(|result|
+        fstar!("$result == Spec.Utils.v_G $input"))
+    )]
     #[inline(always)]
     fn G(input: &[u8]) -> [u8; G_DIGEST_SIZE] {
         let mut digest = [0u8; G_DIGEST_SIZE];
@@ -74,6 +77,9 @@ pub(crate) mod portable {
         digest
     }
 
+    #[cfg_attr(hax,hax_lib::ensures(|result|
+        fstar!("$result == Spec.Utils.v_H $input"))
+    )]
     #[inline(always)]
     fn H(input: &[u8]) -> [u8; H_DIGEST_SIZE] {
         let mut digest = [0u8; H_DIGEST_SIZE];
@@ -81,6 +87,9 @@ pub(crate) mod portable {
         digest
     }
 
+    #[cfg_attr(hax,hax_lib::ensures(|result|
+        fstar!("$result == Spec.Utils.v_PRF $LEN $input"))
+    )]
     #[inline(always)]
     fn PRF<const LEN: usize>(input: &[u8]) -> [u8; LEN] {
         let mut digest = [0u8; LEN];
@@ -189,6 +198,9 @@ pub(crate) mod avx2 {
         shake128_state: KeccakState,
     }
 
+    #[cfg_attr(hax,hax_lib::ensures(|result|
+        fstar!("$result == Spec.Utils.v_G $input"))
+    )]
     #[inline(always)]
     fn G(input: &[u8]) -> [u8; G_DIGEST_SIZE] {
         let mut digest = [0u8; G_DIGEST_SIZE];
@@ -196,6 +208,9 @@ pub(crate) mod avx2 {
         digest
     }
 
+    #[cfg_attr(hax,hax_lib::ensures(|result|
+        fstar!("$result == Spec.Utils.v_H $input"))
+    )]
     #[inline(always)]
     fn H(input: &[u8]) -> [u8; H_DIGEST_SIZE] {
         let mut digest = [0u8; H_DIGEST_SIZE];
@@ -203,6 +218,9 @@ pub(crate) mod avx2 {
         digest
     }
 
+    #[cfg_attr(hax,hax_lib::ensures(|result|
+        fstar!("$result == Spec.Utils.v_PRF $LEN $input"))
+    )]
     #[inline(always)]
     fn PRF<const LEN: usize>(input: &[u8]) -> [u8; LEN] {
         let mut digest = [0u8; LEN];
@@ -407,6 +425,9 @@ pub(crate) mod neon {
         shake128_state: [KeccakState; 2],
     }
 
+    #[cfg_attr(hax,hax_lib::ensures(|result|
+        fstar!("$result == Spec.Utils.v_G $input"))
+    )]
     #[inline(always)]
     fn G(input: &[u8]) -> [u8; G_DIGEST_SIZE] {
         let mut digest = [0u8; G_DIGEST_SIZE];
@@ -414,6 +435,9 @@ pub(crate) mod neon {
         digest
     }
 
+    #[cfg_attr(hax,hax_lib::ensures(|result|
+        fstar!("$result == Spec.Utils.v_H $input"))
+    )]
     #[inline(always)]
     fn H(input: &[u8]) -> [u8; H_DIGEST_SIZE] {
         let mut digest = [0u8; H_DIGEST_SIZE];
@@ -421,6 +445,9 @@ pub(crate) mod neon {
         digest
     }
 
+    #[cfg_attr(hax,hax_lib::ensures(|result|
+        fstar!("$result == Spec.Utils.v_PRF $LEN $input"))
+    )]
     #[inline(always)]
     fn PRF<const LEN: usize>(input: &[u8]) -> [u8; LEN] {
         let mut digest = [0u8; LEN];
